(*  Title:      HOL/Real_Vector_Spaces.thy
    Author:     Brian Huffman
    Author:     Johannes HÃ¶lzl
*)

section \<open>Vector Spaces and Algebras over the Complexs\<close>

theory Complex_Vector_Spaces              
imports Complex_Main "HOL.Topological_Spaces" "HOL.Vector_Spaces"
begin                                   

subsection \<open>Complex vector spaces\<close>

class scaleC =
  fixes scaleC :: "complex \<Rightarrow> 'a \<Rightarrow> 'a" (infixr "*\<^sub>C" 75)
begin

abbreviation divideC :: "'a \<Rightarrow> complex \<Rightarrow> 'a"  (infixl "'/\<^sub>C" 70)
  where "x /\<^sub>C r \<equiv> inverse r *\<^sub>C x"

end

class complex_vector = scaleC + ab_group_add +
  assumes scaleC_add_right: "a *\<^sub>C (x + y) = a *\<^sub>C x + a *\<^sub>C y"
  and scaleC_add_left: "(a + b) *\<^sub>C x = a *\<^sub>C x + b *\<^sub>C x"
  and scaleC_scaleC: "a *\<^sub>C b *\<^sub>C x = (a * b) *\<^sub>C x"
  and scaleC_one: "1 *\<^sub>C x = x"

class complex_algebra = complex_vector + ring +
  assumes mult_scaleC_left [simp]: "a *\<^sub>C x * y = a *\<^sub>C (x * y)"
    and mult_scaleC_right [simp]: "x * a *\<^sub>C y = a *\<^sub>C (x * y)"

class complex_algebra_1 = complex_algebra + ring_1

class complex_div_algebra = complex_algebra_1 + division_ring

class complex_field = complex_div_algebra + field

instantiation complex :: complex_field
begin

definition complex_scaleC_def [simp]: "scaleC a x = a * x"

instance
  by standard (simp_all add: algebra_simps)

end

locale linear = Vector_Spaces.linear "scaleC::_\<Rightarrow>_\<Rightarrow>'a::complex_vector" "scaleC::_\<Rightarrow>_\<Rightarrow>'b::complex_vector"
begin

lemmas scaleC = scale

end

global_interpretation complex_vector?: vector_space "scaleC :: complex \<Rightarrow> 'a \<Rightarrow> 'a :: complex_vector"
  rewrites "Vector_Spaces.linear (*\<^sub>C) (*\<^sub>C) = linear"
    and "Vector_Spaces.linear (*) (*\<^sub>C) = linear"
  defines dependent_raw_def: dependent = complex_vector.dependent
    and representation_raw_def: representation = complex_vector.representation
    and subspace_raw_def: subspace = complex_vector.subspace
    and span_raw_def: span = complex_vector.span
    and extend_basis_raw_def: extend_basis = complex_vector.extend_basis
    and dim_raw_def: dim = complex_vector.dim
proof unfold_locales
  show "Vector_Spaces.linear (*\<^sub>C) (*\<^sub>C) = linear" "Vector_Spaces.linear (*) (*\<^sub>C) = linear"
    by (force simp: linear_def complex_scaleC_def[abs_def])+
qed (use scaleC_add_right scaleC_add_left scaleC_scaleC scaleC_one in auto)

hide_const (open)\<comment> \<open>locale constants\<close>
  complex_vector.dependent
  complex_vector.independent
  complex_vector.representation
  complex_vector.subspace
  complex_vector.span
  complex_vector.extend_basis
  complex_vector.dim


global_interpretation complex_vector?: vector_space_pair "scaleC::_\<Rightarrow>_\<Rightarrow>'a::complex_vector" "scaleC::_\<Rightarrow>_\<Rightarrow>'b::complex_vector"
  rewrites  "Vector_Spaces.linear (*\<^sub>C) (*\<^sub>C) = linear"
    and "Vector_Spaces.linear (*) (*\<^sub>C) = linear"
  defines construct_raw_def: construct = complex_vector.construct
proof unfold_locales
  show "Vector_Spaces.linear (*) (*\<^sub>C) = linear"
  unfolding linear_def complex_scaleC_def by auto
qed (auto simp: linear_def)

hide_const (open)\<comment> \<open>locale constants\<close>
  complex_vector.construct

lemma linear_compose: "linear f \<Longrightarrow> linear g \<Longrightarrow> linear (g \<circ> f)"
  unfolding linear_def by (rule Vector_Spaces.linear_compose)

text \<open>Recover original theorem names\<close>

lemmas scaleC_left_commute = complex_vector.scale_left_commute
lemmas scaleC_zero_left = complex_vector.scale_zero_left
lemmas scaleC_minus_left = complex_vector.scale_minus_left
lemmas scaleC_diff_left = complex_vector.scale_left_diff_distrib
lemmas scaleC_sum_left = complex_vector.scale_sum_left
lemmas scaleC_zero_right = complex_vector.scale_zero_right
lemmas scaleC_minus_right = complex_vector.scale_minus_right
lemmas scaleC_diff_right = complex_vector.scale_right_diff_distrib
lemmas scaleC_sum_right = complex_vector.scale_sum_right
lemmas scaleC_eq_0_iff = complex_vector.scale_eq_0_iff
lemmas scaleC_left_imp_eq = complex_vector.scale_left_imp_eq
lemmas scaleC_right_imp_eq = complex_vector.scale_right_imp_eq
lemmas scaleC_cancel_left = complex_vector.scale_cancel_left
lemmas scaleC_cancel_right = complex_vector.scale_cancel_right

lemma [field_simps]:
  "c \<noteq> 0 \<Longrightarrow> a = b /\<^sub>C c \<longleftrightarrow> c *\<^sub>C a = b"
  "c \<noteq> 0 \<Longrightarrow> b /\<^sub>C c = a \<longleftrightarrow> b = c *\<^sub>C a"
  "c \<noteq> 0 \<Longrightarrow> a + b /\<^sub>C c = (c *\<^sub>C a + b) /\<^sub>C c"
  "c \<noteq> 0 \<Longrightarrow> a /\<^sub>C c + b = (a + c *\<^sub>C b) /\<^sub>C c"
  "c \<noteq> 0 \<Longrightarrow> a - b /\<^sub>C c = (c *\<^sub>C a - b) /\<^sub>C c"
  "c \<noteq> 0 \<Longrightarrow> a /\<^sub>C c - b = (a - c *\<^sub>C b) /\<^sub>C c"
  "c \<noteq> 0 \<Longrightarrow> - (a /\<^sub>C c) + b = (- a + c *\<^sub>C b) /\<^sub>C c"
  "c \<noteq> 0 \<Longrightarrow> - (a /\<^sub>C c) - b = (- a - c *\<^sub>C b) /\<^sub>C c"
  for a b :: "'a :: complex_vector"
  by (auto simp add: scaleC_add_right scaleC_add_left scaleC_diff_right scaleC_diff_left)


text \<open>Legacy names\<close>

lemmas scaleC_left_distrib = scaleC_add_left
lemmas scaleC_right_distrib = scaleC_add_right
lemmas scaleC_left_diff_distrib = scaleC_diff_left
lemmas scaleC_right_diff_distrib = scaleC_diff_right

lemmas linear_injective_0 = linear_inj_iff_eq_0
  and linear_injective_on_subspace_0 = linear_inj_on_iff_eq_0
  and linear_cmul = linear_scale
  and linear_scaleC = linear_scale_self
  and subspace_mul = subspace_scale
  and span_linear_image = linear_span_image
  and span_0 = span_zero
  and span_mul = span_scale
  and injective_scaleC = injective_scale

lemma scaleC_minus1_left [simp]: "scaleC (-1) x = - x"
  for x :: "'a::complex_vector"
  using scaleC_minus_left [of 1 x] by simp

lemma scaleC_2:
  fixes x :: "'a::complex_vector"
  shows "scaleC 2 x = x + x"
  unfolding one_add_one [symmetric] scaleC_left_distrib by simp

lemma scaleC_half_double [simp]:
  fixes a :: "'a::complex_vector"
  shows "(1 / 2) *\<^sub>C (a + a) = a"
proof -
  have "\<And>r. r *\<^sub>C (a + a) = (r * 2) *\<^sub>C a"
    by (metis scaleC_2 scaleC_scaleC)
  then show ?thesis
    by simp
qed

lemma linear_scale_complex:
  fixes r::complex shows "linear f \<Longrightarrow> f (r * b) = r * f b"
  using linear_scale by fastforce

interpretation scaleC_left: additive "(\<lambda>a. scaleC a x :: 'a::complex_vector)"
  by standard (rule scaleC_left_distrib)

interpretation scaleC_right: additive "(\<lambda>x. scaleC a x :: 'a::complex_vector)"
  by standard (rule scaleC_right_distrib)

lemma nonzero_inverse_scaleC_distrib:
  "a \<noteq> 0 \<Longrightarrow> x \<noteq> 0 \<Longrightarrow> inverse (scaleC a x) = scaleC (inverse a) (inverse x)"
  for x :: "'a::complex_div_algebra"
  by (rule inverse_unique) simp

lemma inverse_scaleC_distrib: "inverse (scaleC a x) = scaleC (inverse a) (inverse x)"
  for x :: "'a::{complex_div_algebra,division_ring}"
  by (metis inverse_zero nonzero_inverse_scaleC_distrib scale_eq_0_iff)

lemmas sum_constant_scaleC = complex_vector.sum_constant_scale\<comment> \<open>legacy name\<close>

named_theorems vector_add_divide_simps "to simplify sums of scaled vectors"

lemma [vector_add_divide_simps]:
  "v + (b / z) *\<^sub>C w = (if z = 0 then v else (z *\<^sub>C v + b *\<^sub>C w) /\<^sub>C z)"
  "a *\<^sub>C v + (b / z) *\<^sub>C w = (if z = 0 then a *\<^sub>C v else ((a * z) *\<^sub>C v + b *\<^sub>C w) /\<^sub>C z)"
  "(a / z) *\<^sub>C v + w = (if z = 0 then w else (a *\<^sub>C v + z *\<^sub>C w) /\<^sub>C z)"
  "(a / z) *\<^sub>C v + b *\<^sub>C w = (if z = 0 then b *\<^sub>C w else (a *\<^sub>C v + (b * z) *\<^sub>C w) /\<^sub>C z)"
  "v - (b / z) *\<^sub>C w = (if z = 0 then v else (z *\<^sub>C v - b *\<^sub>C w) /\<^sub>C z)"
  "a *\<^sub>C v - (b / z) *\<^sub>C w = (if z = 0 then a *\<^sub>C v else ((a * z) *\<^sub>C v - b *\<^sub>C w) /\<^sub>C z)"
  "(a / z) *\<^sub>C v - w = (if z = 0 then -w else (a *\<^sub>C v - z *\<^sub>C w) /\<^sub>C z)"
  "(a / z) *\<^sub>C v - b *\<^sub>C w = (if z = 0 then -b *\<^sub>C w else (a *\<^sub>C v - (b * z) *\<^sub>C w) /\<^sub>C z)"
  for v :: "'a :: complex_vector"
  by (simp_all add: divide_inverse_commute scaleC_add_right scaleC_diff_right)


lemma eq_vector_fraction_iff [vector_add_divide_simps]:
  fixes x :: "'a :: complex_vector"
  shows "(x = (u / v) *\<^sub>C a) \<longleftrightarrow> (if v=0 then x = 0 else v *\<^sub>C x = u *\<^sub>C a)"
by auto (metis (no_types) divide_eq_1_iff divide_inverse_commute scaleC_one scaleC_scaleC)

lemma vector_fraction_eq_iff [vector_add_divide_simps]:
  fixes x :: "'a :: complex_vector"
  shows "((u / v) *\<^sub>C a = x) \<longleftrightarrow> (if v=0 then x = 0 else u *\<^sub>C a = v *\<^sub>C x)"
by (metis eq_vector_fraction_iff)

lemma complex_vector_affinity_eq:
  fixes x :: "'a :: complex_vector"
  assumes m0: "m \<noteq> 0"
  shows "m *\<^sub>C x + c = y \<longleftrightarrow> x = inverse m *\<^sub>C y - (inverse m *\<^sub>C c)"
    (is "?lhs \<longleftrightarrow> ?rhs")
proof
  assume ?lhs
  then have "m *\<^sub>C x = y - c" by (simp add: field_simps)
  then have "inverse m *\<^sub>C (m *\<^sub>C x) = inverse m *\<^sub>C (y - c)" by simp
  then show "x = inverse m *\<^sub>C y - (inverse m *\<^sub>C c)"
    using m0
  by (simp add: scaleC_diff_right)
next
  assume ?rhs
  with m0 show "m *\<^sub>C x + c = y"
    by (simp add: scaleC_diff_right)
qed

lemma complex_vector_eq_affinity: "m \<noteq> 0 \<Longrightarrow> y = m *\<^sub>C x + c \<longleftrightarrow> inverse m *\<^sub>C y - (inverse m *\<^sub>C c) = x"
  for x :: "'a::complex_vector"
  using complex_vector_affinity_eq[where m=m and x=x and y=y and c=c]
  by metis

lemma scaleC_eq_iff [simp]: "b + u *\<^sub>C a = a + u *\<^sub>C b \<longleftrightarrow> a = b \<or> u = 1"
  for a :: "'a::complex_vector"
proof (cases "u = 1")
  case True
  then show ?thesis by auto
next
  case False
  have "a = b" if "b + u *\<^sub>C a = a + u *\<^sub>C b"
  proof -
    from that have "(u - 1) *\<^sub>C a = (u - 1) *\<^sub>C b"
      by (simp add: algebra_simps)
    with False show ?thesis
      by auto
  qed
  then show ?thesis by auto
qed

lemma scaleC_collapse [simp]: "(1 - u) *\<^sub>C a + u *\<^sub>C a = a"
  for a :: "'a::complex_vector"
  by (simp add: algebra_simps)


subsection \<open>Embedding of the Complexs into any \<open>complex_algebra_1\<close>: \<open>of_complex\<close>\<close>

definition of_complex :: "complex \<Rightarrow> 'a::complex_algebra_1"
  where "of_complex r = scaleC r 1"

lemma scaleC_conv_of_complex: "scaleC r x = of_complex r * x"
  by (simp add: of_complex_def)

lemma of_complex_0 [simp]: "of_complex 0 = 0"
  by (simp add: of_complex_def)

lemma of_complex_1 [simp]: "of_complex 1 = 1"
  by (simp add: of_complex_def)

lemma of_complex_add [simp]: "of_complex (x + y) = of_complex x + of_complex y"
  by (simp add: of_complex_def scaleC_left_distrib)

lemma of_complex_minus [simp]: "of_complex (- x) = - of_complex x"
  by (simp add: of_complex_def)

lemma of_complex_diff [simp]: "of_complex (x - y) = of_complex x - of_complex y"
  by (simp add: of_complex_def scaleC_left_diff_distrib)

lemma of_complex_mult [simp]: "of_complex (x * y) = of_complex x * of_complex y"
  by (simp add: of_complex_def)

lemma of_complex_sum[simp]: "of_complex (sum f s) = (\<Sum>x\<in>s. of_complex (f x))"
  by (induct s rule: infinite_finite_induct) auto

lemma of_complex_prod[simp]: "of_complex (prod f s) = (\<Prod>x\<in>s. of_complex (f x))"
  by (induct s rule: infinite_finite_induct) auto

lemma nonzero_of_complex_inverse:
  "x \<noteq> 0 \<Longrightarrow> of_complex (inverse x) = inverse (of_complex x :: 'a::complex_div_algebra)"
  by (simp add: of_complex_def nonzero_inverse_scaleC_distrib)

lemma of_complex_inverse [simp]:
  "of_complex (inverse x) = inverse (of_complex x :: 'a::{complex_div_algebra,division_ring})"
  by (simp add: of_complex_def inverse_scaleC_distrib)

lemma nonzero_of_complex_divide:
  "y \<noteq> 0 \<Longrightarrow> of_complex (x / y) = (of_complex x / of_complex y :: 'a::complex_field)"
  by (simp add: divide_inverse nonzero_of_complex_inverse)

lemma of_complex_divide [simp]:
  "of_complex (x / y) = (of_complex x / of_complex y :: 'a::complex_div_algebra)"
  by (simp add: divide_inverse)

lemma of_complex_power [simp]:
  "of_complex (x ^ n) = (of_complex x :: 'a::{complex_algebra_1}) ^ n"
  by (induct n) simp_all

lemma of_complex_power_int [simp]:
  "of_complex (power_int x n) = power_int (of_complex x :: 'a :: {complex_div_algebra,division_ring}) n"
  by (auto simp: power_int_def)

lemma of_complex_eq_iff [simp]: "of_complex x = of_complex y \<longleftrightarrow> x = y"
  by (simp add: of_complex_def)

lemma inj_of_complex: "inj of_complex"
  by (auto intro: injI)

lemmas of_complex_eq_0_iff [simp] = of_complex_eq_iff [of _ 0, simplified]
lemmas of_complex_eq_1_iff [simp] = of_complex_eq_iff [of _ 1, simplified]

lemma minus_of_complex_eq_of_complex_iff [simp]: "-of_complex x = of_complex y \<longleftrightarrow> -x = y"
  using of_complex_eq_iff[of "-x" y] by (simp only: of_complex_minus)

lemma of_complex_eq_minus_of_complex_iff [simp]: "of_complex x = -of_complex y \<longleftrightarrow> x = -y"
  using of_complex_eq_iff[of x "-y"] by (simp only: of_complex_minus)

lemma of_complex_eq_id [simp]: "of_complex = (id :: complex \<Rightarrow> complex)"
  by (rule ext) (simp add: of_complex_def)

text \<open>Collapse nested embeddings.\<close>
lemma of_complex_of_nat_eq [simp]: "of_complex (of_nat n) = of_nat n"
  by (induct n) auto

lemma of_complex_of_int_eq [simp]: "of_complex (of_int z) = of_int z"
  by (cases z rule: int_diff_cases) simp

lemma of_complex_numeral [simp]: "of_complex (numeral w) = numeral w"
  using of_complex_of_int_eq [of "numeral w"] by simp

lemma of_complex_neg_numeral [simp]: "of_complex (- numeral w) = - numeral w"
  using of_complex_of_int_eq [of "- numeral w"] by simp

lemma numeral_power_int_eq_of_complex_cancel_iff [simp]:
  "power_int (numeral x) n = (of_complex y :: 'a :: {complex_div_algebra, division_ring}) \<longleftrightarrow>
     power_int (numeral x) n = y"
proof -
  have "power_int (numeral x) n = (of_complex (power_int (numeral x) n) :: 'a)"
    by simp
  also have "\<dots> = of_complex y \<longleftrightarrow> power_int (numeral x) n = y"
    by (subst of_complex_eq_iff) auto
  finally show ?thesis .
qed

lemma of_complex_eq_numeral_power_int_cancel_iff [simp]:
  "(of_complex y :: 'a :: {complex_div_algebra, division_ring}) = power_int (numeral x) n \<longleftrightarrow>
     y = power_int (numeral x) n"
  by (subst (1 2) eq_commute) simp

lemma of_complex_eq_of_complex_power_int_cancel_iff [simp]:
  "power_int (of_complex b :: 'a :: {complex_div_algebra, division_ring}) w = of_complex x \<longleftrightarrow>
     power_int b w = x"
  by (metis of_complex_power_int of_complex_eq_iff)

lemma of_complex_in_Ints_iff [simp]: "of_complex x \<in> \<int> \<longleftrightarrow> x \<in> \<int>"
proof safe
  fix x assume "(of_complex x :: 'a) \<in> \<int>"
  then obtain n where "(of_complex x :: 'a) = of_int n"
    by (auto simp: Ints_def)
  also have "of_int n = of_complex (real_of_int n)"
    by simp
  finally have "x = real_of_int n"
    by (subst (asm) of_complex_eq_iff)
  thus "x \<in> \<int>"
    by auto
qed (auto simp: Ints_def)

lemma Ints_of_complex [intro]: "x \<in> \<int> \<Longrightarrow> of_complex x \<in> \<int>"
  by simp


text \<open>Every complex algebra has characteristic zero.\<close>
instance complex_algebra_1 < ring_char_0
proof
  from inj_of_complex inj_of_nat have "inj (of_complex \<circ> of_nat)"
    by (rule inj_compose)
  then show "inj (of_nat :: nat \<Rightarrow> 'a)"
    by (simp add: comp_def)
qed

lemma fraction_scaleC_times [simp]:
  fixes a :: "'a::complex_algebra_1"
  shows "(numeral u / numeral v) *\<^sub>C (numeral w * a) = (numeral u * numeral w / numeral v) *\<^sub>C a"
by (metis (no_types, lifting) of_complex_numeral scaleC_conv_of_complex scaleC_scaleC times_divide_eq_left)

lemma inverse_scaleC_times [simp]:
  fixes a :: "'a::complex_algebra_1"
  shows "(1 / numeral v) *\<^sub>C (numeral w * a) = (numeral w / numeral v) *\<^sub>C a"
by (metis divide_inverse_commute inverse_eq_divide of_complex_numeral scaleC_conv_of_complex scaleC_scaleC)

lemma scaleC_times [simp]:
  fixes a :: "'a::complex_algebra_1"
  shows "(numeral u) *\<^sub>C (numeral w * a) = (numeral u * numeral w) *\<^sub>C a"
by (simp add: scaleC_conv_of_complex)

instance complex_field < field_char_0 ..


subsection \<open>The Set of Complex Numbers\<close>

definition Complexs :: "'a::complex_algebra_1 set"  ("\<complex>")
  where "\<complex> = range of_complex"

lemma Complexs_of_complex [simp]: "of_complex r \<in> \<complex>"
  by (simp add: Complexs_def)

lemma Complexs_of_int [simp]: "of_int z \<in> \<complex>"
  by (subst of_complex_of_int_eq [symmetric], rule Complexs_of_complex)

lemma Complexs_of_nat [simp]: "of_nat n \<in> \<complex>"
  by (subst of_complex_of_nat_eq [symmetric], rule Complexs_of_complex)

lemma Complexs_numeral [simp]: "numeral w \<in> \<complex>"
  by (subst of_complex_numeral [symmetric], rule Complexs_of_complex)

lemma Complexs_0 [simp]: "0 \<in> \<complex>" and Complexs_1 [simp]: "1 \<in> \<complex>"
  by (simp_all add: Complexs_def)

lemma Complexs_add [simp]: "a \<in> \<complex> \<Longrightarrow> b \<in> \<complex> \<Longrightarrow> a + b \<in> \<complex>"
  by (metis (no_types, hide_lams) Complexs_def Complexs_of_complex imageE of_complex_add)

lemma Complexs_minus [simp]: "a \<in> \<complex> \<Longrightarrow> - a \<in> \<complex>"
  by (auto simp: Complexs_def)

lemma Complexs_minus_iff [simp]: "- a \<in> \<complex> \<longleftrightarrow> a \<in> \<complex>"
  using Complexs_minus by fastforce

lemma Complexs_diff [simp]: "a \<in> \<complex> \<Longrightarrow> b \<in> \<complex> \<Longrightarrow> a - b \<in> \<complex>"
  by (metis Complexs_add Complexs_minus_iff add_uminus_conv_diff)

lemma Complexs_mult [simp]: "a \<in> \<complex> \<Longrightarrow> b \<in> \<complex> \<Longrightarrow> a * b \<in> \<complex>"
  by (metis (no_types, lifting) Complexs_def Complexs_of_complex imageE of_complex_mult)

lemma nonzero_Complexs_inverse: "a \<in> \<complex> \<Longrightarrow> a \<noteq> 0 \<Longrightarrow> inverse a \<in> \<complex>"
  for a :: "'a::complex_div_algebra"
  by (metis Complexs_def Complexs_of_complex imageE of_complex_inverse)

lemma Complexs_inverse: "a \<in> \<complex> \<Longrightarrow> inverse a \<in> \<complex>"
  for a :: "'a::{complex_div_algebra,division_ring}"
  using nonzero_Complexs_inverse by fastforce

lemma Complexs_inverse_iff [simp]: "inverse x \<in> \<complex> \<longleftrightarrow> x \<in> \<complex>"
  for x :: "'a::{complex_div_algebra,division_ring}"
  by (metis Complexs_inverse inverse_inverse_eq)

lemma nonzero_Complexs_divide: "a \<in> \<complex> \<Longrightarrow> b \<in> \<complex> \<Longrightarrow> b \<noteq> 0 \<Longrightarrow> a / b \<in> \<complex>"
  for a b :: "'a::complex_field"
  by (simp add: divide_inverse)

lemma Complexs_divide [simp]: "a \<in> \<complex> \<Longrightarrow> b \<in> \<complex> \<Longrightarrow> a / b \<in> \<complex>"
  for a b :: "'a::{complex_field,field}"
  using nonzero_Complexs_divide by fastforce

lemma Complexs_power [simp]: "a \<in> \<complex> \<Longrightarrow> a ^ n \<in> \<complex>"
  for a :: "'a::complex_algebra_1"
  by (metis Complexs_def Complexs_of_complex imageE of_complex_power)

lemma Complexs_cases [cases set: Complexs]:
  assumes "q \<in> \<complex>"
  obtains (of_complex) r where "q = of_complex r"
  unfolding Complexs_def
proof -
  from \<open>q \<in> \<complex>\<close> have "q \<in> range of_complex" unfolding Complexs_def .
  then obtain r where "q = of_complex r" ..
  then show thesis ..
qed

lemma sum_in_Complexs [intro,simp]: "(\<And>i. i \<in> s \<Longrightarrow> f i \<in> \<complex>) \<Longrightarrow> sum f s \<in> \<complex>"
proof (induct s rule: infinite_finite_induct)
  case infinite
  then show ?case by (metis Complexs_0 sum.infinite)
qed simp_all

lemma prod_in_Complexs [intro,simp]: "(\<And>i. i \<in> s \<Longrightarrow> f i \<in> \<complex>) \<Longrightarrow> prod f s \<in> \<complex>"
proof (induct s rule: infinite_finite_induct)
  case infinite
  then show ?case by (metis Complexs_1 prod.infinite)
qed simp_all

lemma Complexs_induct [case_names of_complex, induct set: Complexs]:
  "q \<in> \<complex> \<Longrightarrow> (\<And>r. P (of_complex r)) \<Longrightarrow> P q"
  by (rule Complexs_cases) auto


subsection \<open>Ordered complex vector spaces\<close>
(* TODO *)


subsection \<open>Complex normed vector spaces\<close>

 (* TODO *)


end
